[C$] Optimize the parser stobj.
Deepen the stobj by using a stobj array for the sequence of read and unread
characters.

books/kestrel/c/syntax/parser.lisp
@@ -510,13 +510,10 @@
      that fix their inputs and unconditionally return typed outputs.
      The use of a stobj is an optimization for speed:
      conceptually, the parser state could be defined as a @(tsee fty::defprod),
-     and in fact it was defined like that in previous versions of the parser.
-     The description below of the parser state treats the parser state
-     as if it were defined via @(tsee fty::defprod), not as a stobj;
-     at the end, we explain how the stobj represents that parser state.")
+     and in fact it was defined like that in previous versions of the parser.")
    (xdoc::p
-    "The primary component of a parser state
-     is the input sequence @('bytes') of bytes remaining,
+    "The first component of the parser state is
+     the input sequence @('bytes') of bytes remaining,
      which initially comes from a file (see @(see files)).
      Bytes are read and removed from this component,
      and turned into characters.")
@@ -526,97 +523,87 @@
      i.e. putting them back into the parser state.
      But since we have already turned bytes into characters,
      we do not want to put back the bytes:
-     thus, the @('chars-unread') component of the parser state
-     contains a list of characters that have been put back, in character form;
+     thus, we keep, as part of the parser state
+     (the exact representation is explained later),
+     a sequence of unread characters,
+     i.e. characters that have been and then put back (i.e. unread),
+     in character form;
      the form is natural numbers, i.e. Unicode code points.
-     The list is initially empty.
-     When non-empty, it must be thought of
+     The sequence is initially empty.
+     When non-empty, it can be thought of
      as preceding the @('bytes') byte list.
-     If the list is not empty,
+     If the sequence of unread characters is not empty,
      the next character will be read directly from that list,
      not from the byte list.")
    (xdoc::p
     "To avoid putting back the wrong character by mistake,
      i.e. a character that was not actually read,
-     we use the @('chars-read') component of the parser state
+     the parser state also includes a sequence of
+     all the characters read so far and that have not been unread
+     (the exact representation is explained later),
      to keep track of which characters have been read and could be unread.
      Thus, every time we read a character,
-     we add it to the @('chars-read') list,
-     which can be visualized, reversed, to the left of
-     the @('chars-unread') and @('bytes') lists:")
+     we add it to the sequence of read characters,
+     which can be visualized to the left of
+     the sequence of unread characters and the @('bytes') list:")
    (xdoc::codeblock
     "+----------+    read    +--------+-------+"
     "| chars    |   <-----   | chars  | bytes |"
-    "| read     |            | unread |       |"
-    "| reversed |   ----->   |        |       |"
+    "| read     |   ----->   | unread |       |"
     "+----------+   unread   +--------+-------+")
    (xdoc::p
     "The reading of a character moves the character from right to left,
-     from the @('chars-unread') list to the reversed @('chars-read') list
-     if @('chars-unread') is not empty,
-     or from the @('bytes') list to the reversed @('chars-read') list
+     from the sequence of unread characters
+     to the sequence of read characters
+     if the sequence of unread characters is not empty,
+     or from the @('bytes') list to the sequence of read characters
      where one or more bytes are UTF-8-decoded into the character.")
    (xdoc::p
     "When a character is unread, it is moved from left to right,
-     i.e. from the reversed @('chars-read') list to the @('chars-unread') list.
-     If @('chars-read') is empty, it is an internal error:
+     i.e. from the sequence of read characters
+     to the sequence of unread characters.
+     If the sequence of read characters is empty, it is an internal error:
      if the parser code is correct, this must never happen.")
    (xdoc::p
     "The reading and unreading of characters happens at the lexing level.
      A similar look-ahead happens at the proper parsing level,
-     where the elements of the read and unread lists
+     where the elements of the read and unread sequences
      are not characters but tokens.
-     The parser state has lists @('tokens-read') and @('tokens-unread')
+     The parser state includes
+     a sequence of read tokens and a sequence of unread tokens
+     (the exact representation is explained later),
      whose handling is similar to the ones for characters.
-     The lists can be visualized as follows
-     (there are two different situations, explained after the diagram):")
+     The sequence can be visualized as follows,
+     similarly to characters:")
    (xdoc::codeblock
-    "+----------+----------+    read    +--------+-------+"
-    "| tokens   | chars    |   <-----   | chars  | bytes |"
-    "| read     | read     |            | unread |       |"
-    "| reversed | reversed |   ----->   |        |       |"
-    "+----------+----------+   unread   +--------+-------+"
-    ""
-    "+----------+    read    +--------+--------+-------+"
-    "| tokens   |   <-----   | tokens | chars  | bytes |"
-    "| read     |            | unread | unread |       |"
-    "| reversed |   ----->   |        |        |       |"
-    "+----------+   unread   +--------+--------+-------+")
+    "+----------+    read    +--------+"
+    "| tokens   |   <-----   | tokens |"
+    "| read     |   ----->   | unread |"
+    "+----------+   unread   +--------+")
    (xdoc::p
-    "When a token is successfully read,
-     it is moved left to the reversed @('tokens-read') list,
-     and @('chars-read') is cleared.
-     The reason is that, once a token is read,
-     all the characters read form the token,
-     and there is no need to ever unread them:
-     they have already formed the token.
-     But after reading that token, in order to read the next token,
-     the @('chars-read') list is populated with
-     the characters that are read in order to read the next token.
-     So in general the reversed @('tokens-read') list
-     is at the left of the reversed @('chars-read') list,
-     and the latter is cleared again when another token
-     is added to @('tokens-read').
-     This is the first situation depicted in the diagram above.")
+    "When characters are read to form a token,
+     the token is added to the sequence of read tokens.
+     If the token is unread (i.e. put back),
+     it is moved right to the sequence of unread tokens.
+     When a token is read, if the sequence of unread tokens is not empty,
+     the token is moved from right to left;
+     if instead the sequence of unread tokens is empty,
+     the token is read by reading characters and forming the token.")
    (xdoc::p
-    "Characters are read only as a subroutine of reading tokens.
-     If a token is unread, it is unread just after having been read,
-     with the @('chars-read') list still cleared.
-     The unread token is moved right, added to the @('tokens-unread') list.
-     As more tokens are unread, they are also moved right.
-     As they are read again, they are moved left.
-     This is the second situation depicted in the diagram above.
-     Note that we may have some unread characters,
-     which were read and then unread in the course of reading tokens,
-     so the @('chars-unread') list is
-     between the @('token-unread') and @('bytes') lists.")
-   (xdoc::p
-    "While @('chars-read') is cleared every time a token is read,
-     @('tokens-read') is never cleared.
-     This lets us do some backtracking when needed,
+    "At the end of the parsing,
+     the sequence of read characters contains all the characters read,
+     and the sequence of read tokens contains all the tokens read.
+     That is, the sequences are never cleared.
+     For tokens, this lets us do some backtracking when needed,
      but without saving and copying the whole parser state:
      we just need to keep track of how many tokens must be put back
-     for backtracking.")
+     for backtracking.
+     For characters, in principle we could clear
+     the sequence of read characters once a token is formed,
+     but due to the representation of the sequence in the stobj,
+     it is more time-efficient to never clear the sequence,
+     at the cost of some space inefficiency,
+     but we believe the latter not to be significant.")
    (xdoc::p
     "For reporting errors, it is useful to keep track of
      where in a file the constructs being parsed occur.
@@ -627,23 +614,72 @@
      the position is just one past the last character in the file.
      For read and unread characters,
      since we have already found their position and have moved past it,
-     we store their positions in the @('chars-read') and @('chars-unread').
-     This is why they contain not just characters,
+     we store their positions in the sequences of read and unread characters;
+     so those sequences contain not just characters,
      but @(tsee char+position) pairs.
-     Similarly, for tokens, we also store their spans.")
+     Similarly, for tokens, we also store their spans in the sequences.")
+   (xdoc::p
+    "The sequences of read and unread characters
+     are represented by three stobj components.
+     The @('chars') component consists of
+     the concatenation of the two sequences,
+     read characters then unread characters
+     (as shown in the diagrams above),
+     with additional elements to the right to extend the sequences.
+     The @('chars-read') component is the numbers of characters read,
+     which are in the positions 0 (inclusive) to @('chars-read') (exclusive).
+     When @('chars-read') is 0, there are no read characters,
+     which happens at the beginning.
+     The @('chars-unread') component is the number of characters unread,
+     which are in the positions @('chars-read') (inclusive)
+     to @('chars-read + chars-unread') (exclusive).
+     When @('chars-unread') is 0, there are no unread characters,
+     which happens at the beginning,
+     and every time all the unread characters are read again.
+     This organization lets us move characters between the two sequences
+     just by changing @('char-read') and @('char-unread'),
+     but leaving all the characters stored in the stobj array.
+     The position from @('chars-read + chars-unread') (inclusive)
+     to the end of the array are not part of the sequences,
+     but they are used when extending the sequence of read characters
+     when there are no more unread characters:
+     in this situation, @('chars-unread') is 0,
+     and the next character read from the bytes
+     is stored into position @('chars-read'),
+     which is the same as @('chars-read + chars-unread')
+     since @('chars-unread') is 0.")
+   (xdoc::p
+    "The sequence of read and unread tokens
+     are currently represented by two lists
+     @('tokens-read') and @('tokens-unread'),
+     where the first one must be interpreted in reversed order.
+     We plan to use the same array-and-indices organization
+     of characters for tokens,
+     but the lists organization was our initial one for characters as well,
+     and we are in process of optimizing the stobj.
+     For the lists of tokens, tokens are moved between left and right
+     via @(tsee cons)ing and @(tsee cdr)ing,
+     which explains why the @('tokens-read') list is reversed.
+     The stobj component @('tokens-read-len') is an optimization:
+     it is the same as the @(tsee len) of @('tokens-read'),
+     but it is cached for efficiency.
+     However, that will go away once we change the reprentation
+     to use an array and two indices for read and unread tokens.")
    (xdoc::p
     "To support backtracking,
      we also keep track of zero or more checkpoints,
-     which indicate positions in the @('tokens-read') list.
+     which indicate positions in the sequence of read tokens.
      When a checkpoint is recorded,
-     the current length of @('tokens-read') is stored as a checkpoint,
+     the current length of the sequence is stored as a checkpoint,
      by @(tsee cons)ing it to the @('checkpoints') list.
      Later, the checkpoint can be simply cleared,
      in which case it is simply removed from the list,
      by replacing @('checkpoints') with its @(tsee cdr).
      Alternatively, we can backtrack to the checkpoint,
-     which involves moving tokens from @('tokens-read') to @('tokens-unread')
-     until @('tokens-read') has the length of the checkpoint in question;
+     which involves moving tokens from the sequence of read tokens
+     to the sequence of unread tokens,
+     until the sequence of read tokens has
+     the length of the checkpoint in question;
      then the checkpoint is removed from @('checkpoints') as well.
      That is, we have the ability to backtrack to earlier tokens,
      without having to keep track of how many tokens we have read
@@ -672,24 +708,13 @@
      but that transformation currently does not quite handle
      all of the parser's functions.")
    (xdoc::p
-    "Also for speed, we cache the number of the tokens read so far.
-     The checkpointing and backtracking mechanism described above
-     calculates that length in order to record it as a checkpoint.
-     When there is a significant number of read token, that can take time,
-     as revealed by some profiling.")
-   (xdoc::p
-    "The stobj for the parser state consists of
-     the components described above,
-     but in a stobj instead of a @(tsee fty::defprod).
-     This is a ``shallow'' stobj, because several of the components
-     are still lists that are updated in a non-destructive way.
-     We plan to ``deepen'' the stobj by using arrays and indices
-     to simulate those lists in a more efficient way.")
-   (xdoc::p
     "The definition of the stobj itself is straightforward,
-     but we use a @(tsee make-event) so we can use @(tsee position-init)
-     instead of a term for its value that exposes
-     the internal representation of positions.")
+     but we use a @(tsee make-event) so we can use
+     richer terms for initial values.
+     The initial @('chars') array has length 1,
+     which seems convenient for some fixing theorems,
+     but it is irrelevant because it is resized
+     at the very beginning of parsing.")
    (xdoc::p
     "The @(tsee defstobj) generates an enabled recognizer,
      which we disable after introducing the readers and writers.
@@ -715,7 +740,10 @@
      but they neither fix their inputs
      nor return outputs with unconditional types.
      So we define our own readers and writers that do both things,
-     which we define in terms of the generated ones.
+     which we define in terms of the generated ones
+     (actually, a few readers and writers do not fix their inputs yet,
+     because we need to tweak the definition of the fixer for that,
+     which we plan to do soon).
      The generated ones are enabled,
      but we do not bother disabling them,
      because we are not going to use them anywhere anyhow.
@@ -725,18 +753,19 @@
     "We locally enable @(tsee length) in order for
      the proofs generated by @(tsee defstobj) to go through.
      This is also useful for proofs about our readers and writers;
-     for those, we also locally enable the fixer.")
+     for those, we also locally enable the fixer,
+     and we prove some local theorems that are used there.")
    (xdoc::p
     "By making the parser state a stobj instead of a @(tsee fty::defprod),
      we cannot use the @(':require') feature of @(tsee fty::defprod)
-     to enforce that the two redundant components described above
-     are indeed redundant.
+     to enforce invariants, such as the fact that
+     the @('size') component is derived from others.
      But we can probably use @(tsee defabsstobj) for that,
      which may be also overall a better way to
      ``turn'' a stobj into a @(tsee fty::defprod)-like fixtype;
      we will look into that in the future."))
 
-  ;; needed for DEFSTOBJ and writer proofs:
+  ;; needed for DEFSTOBJ and reader/writer proofs:
 
   (local (in-theory (enable length)))
 
@@ -748,10 +777,14 @@
              :initially nil)
       (position :type (satisfies positionp)
                 :initially ,(position-init))
-      (chars-read :type (satisfies char+position-listp)
-                  :initially nil)
-      (chars-unread :type (satisfies char+position-listp)
-                    :initially nil)
+      (chars :type (array (satisfies char+position-p) (1))
+             :initially ,(make-char+position :char 0
+                                             :position (position-init))
+             :resizable t)
+      (chars-read :type (integer 0 *)
+                  :initially 0)
+      (chars-unread :type (integer 0 *)
+                    :initially 0)
       (tokens-read :type (satisfies token+span-listp)
                    :initially nil)
       (tokens-read-len :type (integer 0 *)
@@ -767,6 +800,7 @@
       :renaming (;; field recognizers:
                  (bytesp raw-parstate->bytes-p)
                  (positionp raw-parstate->position-p)
+                 (charsp raw-parstate->chars-p)
                  (chars-readp raw-parstate->chars-read-p)
                  (chars-unreadp raw-parstate->chars-unread-p)
                  (tokens-readp raw-parstate->tokens-read-p)
@@ -778,6 +812,8 @@
                  ;; field readers:
                  (bytes raw-parstate->bytes)
                  (position raw-parstate->position)
+                 (chars-length raw-parstate->chars-length)
+                 (charsi raw-parstate->char)
                  (chars-read raw-parstate->chars-read)
                  (chars-unread raw-parstate->chars-unread)
                  (tokens-read raw-parstate->tokens-read)
@@ -789,6 +825,8 @@
                  ;; field writers:
                  (update-bytes raw-update-parstate->bytes)
                  (update-position raw-update-parstate->position)
+                 (resize-chars raw-update-parstate->chars-length)
+                 (update-charsi raw-update-parstate->char)
                  (update-chars-read raw-update-parstate->chars-read)
                  (update-chars-unread raw-update-parstate->chars-unread)
                  (update-tokens-read raw-update-parstate->tokens-read)
@@ -821,9 +859,33 @@
     :define t
     :executablep nil)
 
-  ;; needed for readers and writers proofs:
+  ;; needed for reader/writer proofs:
 
   (local (in-theory (enable parstate-fix)))
+
+  (defruled raw-parstate->chars-p-of-resize-list
+    (implies (and (raw-parstate->chars-p chars)
+                  (char+position-p default))
+             (raw-parstate->chars-p (resize-list chars length default)))
+    :induct t
+    :enable (resize-list))
+
+  (defruled char+position-p-of-nth-when-raw-parstate->chars-p
+    (implies (and (raw-parstate->chars-p chars)
+                  (natp i)
+                  (< i (len chars)))
+             (char+position-p (nth i chars)))
+    :induct t
+    :enable (nth len))
+
+  (defruled raw-parstate->chars-p-of-update-nth
+    (implies (raw-parstate->chars-p chars)
+             (equal (raw-parstate->chars-p (update-nth i char chars))
+                    (and (char+position-p char)
+                         (<= (nfix i) (len chars)))))
+    :induct t
+    :enable (update-nth nfix zp len)
+    :prep-books ((include-book "arithmetic-3/top" :dir :system)))
 
   ;; readers:
 
@@ -846,19 +908,40 @@
          :exec (raw-parstate->position parstate))
     :hooks (:fix))
 
+  (define parstate->chars-length (parstate)
+    :returns (length natp)
+    (mbe :logic (if (parstatep parstate)
+                    (raw-parstate->chars-length parstate)
+                  1)
+         :exec (raw-parstate->chars-length parstate))
+    :hooks (:fix))
+
+  (define parstate->char ((i natp) parstate)
+    :guard (< i (parstate->chars-length parstate))
+    :returns (char+pos char+position-p
+                       :hints
+                       (("Goal" :in-theory (enable parstate->chars-length))))
+    (mbe :logic (if (and (parstatep parstate)
+                         (< (nfix i) (parstate->chars-length parstate)))
+                    (raw-parstate->char (nfix i) parstate)
+                  (make-char+position :char 0
+                                      :position (position-init)))
+         :exec (raw-parstate->char i parstate))
+    :guard-hints (("Goal" :in-theory (enable nfix parstate->chars-length))))
+
   (define parstate->chars-read (parstate)
-    :returns (chars-read char+position-listp)
+    :returns (chars-read natp :rule-classes (:rewrite :type-prescription))
     (mbe :logic (if (parstatep parstate)
                     (raw-parstate->chars-read parstate)
-                  nil)
+                  0)
          :exec (raw-parstate->chars-read parstate))
     :hooks (:fix))
 
   (define parstate->chars-unread (parstate)
-    :returns (chars-unread char+position-listp)
+    :returns (chars-unread natp :rule-classes (:rewrite :type-prescription))
     (mbe :logic (if (parstatep parstate)
                     (raw-parstate->chars-unread parstate)
-                  nil)
+                  0)
          :exec (raw-parstate->chars-unread parstate))
     :hooks (:fix))
 
@@ -924,20 +1007,46 @@
       (raw-update-parstate->position (position-fix position) parstate))
     :hooks (:fix))
 
-  (define update-parstate->chars-read ((chars-read char+position-listp)
-                                       parstate)
-    :returns (parstate parstatep)
+  (define update-parstate->chars-length ((length natp) parstate)
+    :returns (parstate parstatep
+                       :hints (("Goal"
+                                :in-theory (enable nfix
+                                                   parstate-fix
+                                                   length))))
     (b* ((parstate (parstate-fix parstate)))
-      (raw-update-parstate->chars-read (char+position-list-fix chars-read)
-                                       parstate))
+      (raw-update-parstate->chars-length (nfix length) parstate))
     :hooks (:fix))
 
-  (define update-parstate->chars-unread ((chars-unread char+position-listp)
-                                         parstate)
+  (define update-parstate->char ((i natp)
+                                 (char+pos char+position-p)
+                                 parstate)
+    :guard (< i (parstate->chars-length parstate))
+    :returns (parstate parstatep
+                       :hints
+                       (("Goal"
+                         :in-theory
+                         (enable update-nth-array
+                                 parstate->chars-length
+                                 raw-parstate->chars-p-of-update-nth))))
+    (b* ((parstate (parstate-fix parstate)))
+      (mbe :logic (if (< (nfix i) (parstate->chars-length parstate))
+                      (raw-update-parstate->char (nfix i)
+                                                 (char+position-fix char+pos)
+                                                 parstate)
+                    parstate)
+           :exec (raw-update-parstate->char i char+pos parstate)))
+    :guard-hints (("Goal" :in-theory (enable parstate->chars-length nfix))))
+
+  (define update-parstate->chars-read ((chars-read natp) parstate)
     :returns (parstate parstatep)
     (b* ((parstate (parstate-fix parstate)))
-      (raw-update-parstate->chars-unread (char+position-list-fix chars-unread)
-                                         parstate))
+      (raw-update-parstate->chars-read (nfix chars-read) parstate))
+    :hooks (:fix))
+
+  (define update-parstate->chars-unread ((chars-unread natp) parstate)
+    :returns (parstate parstatep)
+    (b* ((parstate (parstate-fix parstate)))
+      (raw-update-parstate->chars-unread (nfix chars-unread) parstate))
     :hooks (:fix))
 
   (define update-parstate->tokens-read ((tokens-read token+span-listp)
@@ -983,6 +1092,24 @@
     :hooks (:fix))
 
   ;; readers over writers:
+
+  (defrule parstate->size-of-update-parstate->bytes
+    (equal (parstate->size (update-parstate->bytes bytes parstate))
+           (parstate->size parstate))
+    :enable (parstate->size
+             update-parstate->bytes
+             parstatep
+             parstate-fix
+             length))
+
+  (defrule parstate->size-of-update-parstate->position
+    (equal (parstate->size (update-parstate->position position parstate))
+           (parstate->size parstate))
+    :enable (parstate->size
+             update-parstate->position
+             parstatep
+             parstate-fix
+             length))
 
   (defrule parstate->size-of-update-parstate->tokens-read
     (equal (parstate->size (update-parstate->tokens-read tokens-read parstate))
@@ -1039,14 +1166,21 @@
      and a flag saying whether GCC extensions should be accepted or not,
      the initial parsing state consists of
      the data to parse,
-     no unread characters or tokens,
      no read characters or tokens,
+     no unread characters or tokens,
      the initial file position,
-     and no checkpoints."))
+     and no checkpoints.
+     We also resize the array of characters to the number of data bytes,
+     which is overkill but certainly sufficient
+     (because we will never lex more characters than bytes);
+     if this turns out to be too large,
+     we will pick a different size,
+     but then we may need to resize the array as needed while lexing."))
   (b* ((parstate (update-parstate->bytes data parstate))
        (parstate (update-parstate->position (position-init) parstate))
-       (parstate (update-parstate->chars-read nil parstate))
-       (parstate (update-parstate->chars-unread nil parstate))
+       (parstate (update-parstate->chars-length (len data) parstate))
+       (parstate (update-parstate->chars-read 0 parstate))
+       (parstate (update-parstate->chars-unread 0 parstate))
        (parstate (update-parstate->tokens-read nil parstate))
        (parstate (update-parstate->tokens-read-len 0 parstate))
        (parstate (update-parstate->tokens-unread nil parstate))
@@ -1079,33 +1213,63 @@
 
 ;;;;;;;;;;;;;;;;;;;;;;;;;;;;;;;;;;;;;;;;
 
-; fixtype version of PARSTATE stobj (useful for debugging and testing)
+; Fixtype version of PARSTATE stobj (useful for debugging and testing).
+; This is how the parser state was originally defined,
+; before using a stobj and before caching the size.
 (fty::defprod parstate$
   ((bytes byte-list)
    (position position)
    (chars-read char+position-list)
    (chars-unread char+position-list)
    (tokens-read token+span-list)
-   (tokens-read-len nat)
    (tokens-unread token+span-list)
    (checkpoints nat-list)
-   (gcc bool)
-   (size nat))
+   (gcc bool))
   :prepwork ((local (in-theory (enable nfix)))))
 
-; convert PARSTATE stobj to fixtype value (useful for debugging and testing)
+; Convert PARSTATE stobj to fixtype value (useful for debugging and testing).
+; To construct the lists of read and unread characters,
+; we need to loop through suitable ranges of the character array.
 (define to-parstate$ (parstate)
   (make-parstate$
    :bytes (parstate->bytes parstate)
    :position (parstate->position parstate)
-   :chars-read (parstate->chars-read parstate)
-   :chars-unread (parstate->chars-unread parstate)
+   :chars-read (to-parstate$-chars-read (parstate->chars-read parstate)
+                                        parstate)
+   :chars-unread (to-parstate$-chars-unread (parstate->chars-unread parstate)
+                                            parstate)
    :tokens-read (parstate->tokens-read parstate)
-   :tokens-read-len (parstate->tokens-read-len parstate)
    :tokens-unread (parstate->tokens-unread parstate)
    :checkpoints (parstate->checkpoints parstate)
-   :gcc (parstate->gcc parstate)
-   :size (parstate->size parstate)))
+   :gcc (parstate->gcc parstate))
+
+  :prepwork
+
+  ((define to-parstate$-chars-read ((n natp) parstate)
+     :returns (chars char+position-listp)
+     (b* (((when (zp n)) nil)
+          (i (1- n))
+          ((unless (< i (parstate->chars-length parstate)))
+           (raise "Internal error: chars-read index ~x0 out of bound ~x1."
+                  i (parstate->chars-length parstate))))
+       (cons (parstate->char i parstate)
+             (to-parstate$-chars-read (1- n) parstate))))
+
+   (define to-parstate$-chars-unread ((n natp) parstate)
+     :returns (chars char+position-listp)
+     (b* (((when (zp n)) nil)
+          (i (+ (parstate->chars-read parstate)
+                (- (parstate->chars-unread parstate)
+                   n)))
+          ((unless (>= i 0))
+           (raise "Internal error: chars-unread index ~x0 is negative."
+                  i))
+          ((unless (< i (parstate->chars-length parstate)))
+           (raise "Internal error: chars-unread index ~x0 out of bound ~x1."
+                  i (parstate->chars-length parstate))))
+       (cons (parstate->char i parstate)
+             (to-parstate$-chars-unread (1- n) parstate)))
+     :guard-hints (("Goal" :in-theory (enable natp zp))))))
 
 ;;;;;;;;;;;;;;;;;;;;;;;;;;;;;;;;;;;;;;;;;;;;;;;;;;;;;;;;;;;;;;;;;;;;;;;;;;;;;;;;
 
@@ -1249,18 +1413,29 @@
      the non-existent character just past the end of the file
      (i.e. the position of a character if we added it to the end of the file).")
    (xdoc::p
-    "If a character is read, it is added to the list of read characters.
-     See @(tsee parstate).")
-   (xdoc::p
-    "If some character was put back earlier,
-     we get the character directly from there,
-     removing it from the list;
+    "First we check whether the sequence of unread characters is not empty.
+     If it is not empty, we move a character from that sequence
+     to the sequence of read characters,
+     which amounts to incrementing @('chars-read')
+     and decrementing @('chars-unread'),
+     with no change to the array;
      see @(tsee parstate).
-     There is no change in position in the parser state in this case,
-     because the position is the one at the start of the byte list.
-     Otherwise, we look at the bytes.")
+     We also need to check that the @('size') stobj component is not 0,
+     which should be an invariant but it is not explicated in the stobj,
+     because we also decrement that stobj component,
+     to maintain the invariant.
+     We read the character (and its position)
+     from the array so we can return it,
+     but we need to check that the index (i.e. @('chars-read'))
+     is within the bounds of the array.
+     Maybe we could optimize this check away with suitable invariants,
+     presumably via abstract stobjs;
+     this could also let us optimize away
+     the extra check on @('size') mentioned above.")
    (xdoc::p
-    "If there are no more bytes, we have reached the end of file.
+    "If the sequence of unread characters is empty,
+     we need to read the next character from the bytes.
+     If there are no more bytes, we have reached the end of file.
      We return @('nil'), for no character,
      and we leave the parser state unchanged.")
    (xdoc::p
@@ -1366,13 +1541,19 @@
        (parstate.chars-read (parstate->chars-read parstate))
        (parstate.chars-unread (parstate->chars-unread parstate))
        (parstate.size (parstate->size parstate))
-       ((when (and (consp parstate.chars-unread)
+       ((when (and (> parstate.chars-unread 0)
                    (> parstate.size 0)))
-        (b* ((char+pos (car parstate.chars-unread))
-             (parstate (update-parstate->chars-unread
-                        (cdr parstate.chars-unread) parstate))
-             (parstate (update-parstate->chars-read
-                        (cons char+pos parstate.chars-read) parstate))
+        (b* (((unless (< parstate.chars-read
+                         (parstate->chars-length parstate)))
+              (raise "Internal error: index ~x0 out of bound ~x1."
+                     parstate.chars-read
+                     (parstate->chars-length parstate))
+              (reterr t))
+             (char+pos (parstate->char parstate.chars-read parstate))
+             (parstate (update-parstate->chars-unread (1- parstate.chars-unread)
+                                                      parstate))
+             (parstate (update-parstate->chars-read (1+ parstate.chars-read)
+                                                    parstate))
              (parstate (update-parstate->size (1- parstate.size) parstate)))
           (retok (char+position->char char+pos)
                  (char+position->position char+pos)
@@ -1390,12 +1571,19 @@
         (b* ((parstate (update-parstate->bytes bytes parstate))
              (parstate (update-parstate->position
                         (position-inc-column 1 parstate.position) parstate))
-             (parstate (update-parstate->chars-read
-                        (cons (make-char+position
-                               :char byte
-                               :position parstate.position)
-                              parstate.chars-read)
-                        parstate))
+             ((unless (< parstate.chars-read
+                         (parstate->chars-length parstate)))
+              (raise "Internal error: index ~x0 out of bound ~x1."
+                     parstate.chars-read
+                     (parstate->chars-length parstate))
+              (reterr t))
+             (parstate (update-parstate->char parstate.chars-read
+                                              (make-char+position
+                                               :char byte
+                                               :position parstate.position)
+                                              parstate))
+             (parstate (update-parstate->chars-read (1+ parstate.chars-read)
+                                                    parstate))
              (parstate (update-parstate->size (1- parstate.size) parstate)))
           (retok byte parstate.position parstate)))
        ;; line feed:
@@ -1403,12 +1591,19 @@
         (b* ((parstate (update-parstate->bytes bytes parstate))
              (parstate (update-parstate->position
                         (position-inc-line 1 parstate.position) parstate))
-             (parstate (update-parstate->chars-read
-                        (cons (make-char+position
-                               :char 10
-                               :position parstate.position)
-                              parstate.chars-read)
-                        parstate))
+             ((unless (< parstate.chars-read
+                         (parstate->chars-length parstate)))
+              (raise "Internal error: index ~x0 out of bound ~x1."
+                     parstate.chars-read
+                     (parstate->chars-length parstate))
+              (reterr t))
+             (parstate (update-parstate->char parstate.chars-read
+                                              (make-char+position
+                                               :char 10
+                                               :position parstate.position)
+                                              parstate))
+             (parstate (update-parstate->chars-read (1+ parstate.chars-read)
+                                                    parstate))
              (parstate (update-parstate->size (1- parstate.size) parstate)))
           (retok 10 parstate.position parstate)))
        ;; carriage return:
@@ -1421,12 +1616,19 @@
              (parstate (update-parstate->bytes bytes parstate))
              (parstate (update-parstate->position
                         (position-inc-line 1 parstate.position) parstate))
-             (parstate (update-parstate->chars-read
-                        (cons (make-char+position
-                               :char 10
-                               :position parstate.position)
-                              parstate.chars-read)
-                        parstate))
+             ((unless (< parstate.chars-read
+                         (parstate->chars-length parstate)))
+              (raise "Internal error: index ~x0 out of bound ~x1."
+                     parstate.chars-read
+                     (parstate->chars-length parstate))
+              (reterr t))
+             (parstate (update-parstate->char parstate.chars-read
+                                              (make-char+position
+                                               :char 10
+                                               :position parstate.position)
+                                              parstate))
+             (parstate (update-parstate->chars-read (1+ parstate.chars-read)
+                                                    parstate))
              (parstate (update-parstate->size
                         (- parstate.size count) parstate)))
           (retok 10 parstate.position parstate)))
@@ -1466,12 +1668,19 @@
              (parstate (update-parstate->bytes bytes parstate))
              (parstate (update-parstate->position
                         (position-inc-column 1 parstate.position) parstate))
-             (parstate (update-parstate->chars-read
-                        (cons (make-char+position
-                               :char code
-                               :position parstate.position)
-                              parstate.chars-read)
-                        parstate))
+             ((unless (< parstate.chars-read
+                         (parstate->chars-length parstate)))
+              (raise "Internal error: index ~x0 out of bound ~x1."
+                     parstate.chars-read
+                     (parstate->chars-length parstate))
+              (reterr t))
+             (parstate (update-parstate->char parstate.chars-read
+                                              (make-char+position
+                                               :char code
+                                               :position parstate.position)
+                                              parstate))
+             (parstate (update-parstate->chars-read (1+ parstate.chars-read)
+                                                    parstate))
              (parstate (update-parstate->size (- parstate.size 2) parstate)))
           (retok code parstate.position parstate)))
        ;; 3-byte UTF-8:
@@ -1549,12 +1758,19 @@
              (parstate (update-parstate->bytes bytes parstate))
              (parstate (update-parstate->position
                         (position-inc-column 1 parstate.position) parstate))
-             (parstate (update-parstate->chars-read
-                        (cons (make-char+position
-                               :char code
-                               :position parstate.position)
-                              parstate.chars-read)
-                        parstate))
+             ((unless (< parstate.chars-read
+                         (parstate->chars-length parstate)))
+              (raise "Internal error: index ~x0 out of bound ~x1."
+                     parstate.chars-read
+                     (parstate->chars-length parstate))
+              (reterr t))
+             (parstate (update-parstate->char parstate.chars-read
+                                              (make-char+position
+                                               :char code
+                                               :position parstate.position)
+                                              parstate))
+             (parstate (update-parstate->chars-read (1+ parstate.chars-read)
+                                                    parstate))
              (parstate (update-parstate->size (- parstate.size 3) parstate)))
           (retok code parstate.position parstate)))
        ;; 4-byte UTF-8:
@@ -1658,12 +1874,19 @@
              (parstate (update-parstate->bytes bytes parstate))
              (parstate (update-parstate->position
                         (position-inc-column 1 parstate.position) parstate))
-             (parstate (update-parstate->chars-read
-                        (cons (make-char+position
-                               :char code
-                               :position parstate.position)
-                              parstate.chars-read)
-                        parstate))
+             ((unless (< parstate.chars-read
+                         (parstate->chars-length parstate)))
+              (raise "Internal error: index ~x0 out of bound ~x1."
+                     parstate.chars-read
+                     (parstate->chars-length parstate))
+              (reterr t))
+             (parstate (update-parstate->char parstate.chars-read
+                                              (make-char+position
+                                               :char code
+                                               :position parstate.position)
+                                              parstate))
+             (parstate (update-parstate->chars-read (1+ parstate.chars-read)
+                                                    parstate))
              (parstate (update-parstate->size (- parstate.size 4) parstate)))
           (retok code parstate.position parstate))))
     (reterr-msg :where (position-to-msg parstate.position)
@@ -1706,35 +1929,32 @@
   :long
   (xdoc::topstring
    (xdoc::p
-    "We pop the character from the @('chars-read') stack
-     and we push it onto the @('chars-unread') stack.")
+    "We move the character from the sequence of read characters
+     to the sequence of unread characters,
+     by incrementing @('chars-unread') and decrementing @('chars-read').")
    (xdoc::p
-    "It is an internal error if the @('chars-read') stack is empty.
+    "It is an internal error if @('chars-read') is 0.
      It means that the calling code is wrong.
      In this case, after raising the hard error,
      logically we return a parser state
-     where we push an irrelevant character and position,
+     where we still increment @('chars-unread')
      so that the theorem about @(tsee parsize) holds unconditionally."))
   (b* ((parstate.chars-read (parstate->chars-read parstate))
        (parstate.chars-unread (parstate->chars-unread parstate))
        (parstate.size (parstate->size parstate))
-       ((unless (consp parstate.chars-read))
+       ((unless (> parstate.chars-read 0))
         (raise "Internal error: no character to unread.")
-        (b* ((parstate (update-parstate->chars-unread
-                        (cons (make-char+position
-                               :char 0
-                               :position (irr-position))
-                              parstate.chars-unread)
-                        parstate))
+        (b* ((parstate (update-parstate->chars-unread (1+ parstate.chars-unread)
+                                                      parstate))
              (parstate (update-parstate->size (1+ parstate.size) parstate)))
           parstate))
-       (char+pos (car parstate.chars-read))
-       (parstate (update-parstate->chars-unread
-                  (cons char+pos parstate.chars-unread) parstate))
-       (parstate (update-parstate->chars-read
-                  (cdr parstate.chars-read) parstate))
+       (parstate (update-parstate->chars-read (1- parstate.chars-read)
+                                              parstate))
+       (parstate (update-parstate->chars-unread (1+ parstate.chars-unread)
+                                                parstate))
        (parstate (update-parstate->size (1+ parstate.size) parstate)))
     parstate)
+  :guard-hints (("Goal" :in-theory (enable natp)))
 
   ///
 
@@ -4878,7 +5098,7 @@
                         (cons token+span parstate.tokens-read) parstate))
              (parstate (update-parstate->tokens-read-len
                         (1+ parstate.tokens-read-len) parstate))
-             (parstate (update-parstate->chars-read nil parstate))
+             ;; (parstate (update-parstate->chars-read nil parstate))
              (parstate (update-parstate->size (1- parstate.size) parstate)))
           (retok (token+span->token token+span)
                  (token+span->span token+span)
